src/program_proof/pav/client.v
@@ -3,26 +3,7 @@ From Goose.github_com.mit_pdos.pav Require Import kt.
 
 From Perennial.program_proof.pav Require Import advrpc auditor core classes cryptoffi evidence merkle rpc serde server.
 From Perennial.program_proof Require Import std_proof.
-
-Section invs.
-Context `{!heapGS Σ, !pavG Σ}.
-Definition cli_inv γ : iProp Σ :=
-  ∃ ms,
-  "Hown_maps" ∷ mono_list_auth_own γ (1/2) ms ∗
-  "Hown_entries" ∷ ([∗ list] x ∈ ms,
-    match x with
-    | None => True
-    | Some (_, m_γ) => ∃ m, ghost_map_auth m_γ (1/2) m
-    end) ∗
-  "#His_entry" ∷ (□ ∀ (ep : w64) dig m_γ uid ver val,
-    ("#Hsubmap" ∷ mono_list_idx_own γ (uint.nat ep) (Some (dig, m_γ)) ∗
-    "#Hin_map" ∷ (uid, ver) ↪[m_γ]□ val)
-    -∗
-    (∃ label,
-    "#His_label" ∷ is_vrf uid ver label ∗
-    "#Hhas_mproof" ∷ has_merkp label
-      ((λ x, MapValPre.encodesF (MapValPre.mk x.1 x.2)) <$> val) dig)).
-End invs.
+From Perennial.Helpers Require Import Map.
 
 Module Client.
 Record t :=
@@ -41,37 +22,61 @@ Global Instance eta : Settable _ :=
 Section defs.
 Context `{!heapGS Σ, !pavG Σ}.
 
+Definition map_inv (m : cli_map_ty) (dig : list w8) : iProp Σ :=
+  ([∗ map] k ↦ val ∈ m,
+    ∃ label,
+    "#His_label" ∷ is_vrf k.1 k.2 label ∗
+    "#Hhas_mproof" ∷ has_merkp label
+      ((λ x, MapValPre.encodesF (MapValPre.mk x.1 x.2)) <$> val) dig).
+
+Definition inv γ : iProp Σ :=
+  ∃ ms,
+  "Hown_epochs" ∷ mono_list_auth_own γ (1/2)
+    ((λ (x : option _), (λ y, y.1) <$> x) <$> ms) ∗
+  "Hown_maps" ∷ ([∗ list] x ∈ ms,
+    match x with None => True | Some (m_γ, _, m) =>
+    ghost_map_auth m_γ 1 m end) ∗
+  "#His_maps" ∷ ([∗ list] x ∈ ms,
+    match x with None => True | Some (_, dig, m) => map_inv m dig end).
+
 Definition own (ptr : loc) (obj : t) : iProp Σ :=
   ∃ ms ptr_sd sd_ptrs sd ptr_serv_cli serv_cli sl_serv_sig_pk,
-  (* GS. *)
-  "#Hinv" ∷ inv nroot (cli_inv obj.(γ)) ∗
-  "Hown_maps" ∷ mono_list_auth_own obj.(γ) (1/2) ms ∗
-  "Hown_entries" ∷ ([∗ list] x ∈ ms,
-    match x with
-    | None => True
-    | Some (_, m_γ) => ∃ m, ghost_map_auth m_γ (1/2) m
-    end) ∗
   (* seenDigs. *)
-  "Hown_sd" ∷ own_map ptr_sd (DfracOwn 1) sd_ptrs ∗
-  "Hptr_sd" ∷ ptr ↦[Client :: "seenDigs"] #ptr_sd ∗
-  "Hown_sd_ptrs" ∷ ([∗ map] l;v ∈ sd_ptrs;sd, SigDig.own l v) ∗
-  "%Hagree_sd" ∷ ⌜ (∀ (ep : w64) dig m_γ,
-    ms !! (uint.nat ep) = Some (Some (dig, m_γ)) →
-    (∃ x, sd !! ep = Some x ∧ x.(SigDig.Dig) = dig)) ⌝ ∗
+  "Hown_sd_map" ∷ own_map ptr_sd (DfracOwn 1) sd_ptrs ∗
+  "#Hptr_sd" ∷ ptr ↦[Client :: "seenDigs"]□ #ptr_sd ∗
+  "#Hown_sd" ∷ ([∗ map] l;v ∈ sd_ptrs;sd, SigDig.own l v) ∗
+  "#His_sd" ∷ ([∗ map] x ∈ sd, is_SigDig x obj.(serv_sig_pk)) ∗
+  (* GS. *)
+  "#Hinv" ∷ inv nroot (inv obj.(γ)) ∗
+  "Hown_epochs" ∷ mono_list_auth_own obj.(γ) (1/2)
+    ((λ (x : option _), (λ y, y.1) <$> x) <$> ms) ∗
+  "Hown_maps" ∷ ([∗ list] x ∈ ms,
+    match x with None => True | Some (m_γ, _, m) =>
+    ghost_map_auth m_γ (1/2) m end) ∗
+  "%Hagree_sd" ∷ ([∗ list] ep ↦ x ∈ ms,
+    match x with None => True | Some (_, dig, _) =>
+    ∃ sig,
+    "%Hlook_sd" ∷ ⌜ sd !! (W64 ep) = Some (SigDig.mk (W64 ep) dig sig) ⌝ end) ∗
   (* uid, next_ver, next_epoch. *)
-  "Hptr_uid" ∷ ptr ↦[Client :: "uid"] #obj.(uid) ∗
+  "#Hptr_uid" ∷ ptr ↦[Client :: "uid"]□ #obj.(uid) ∗
   "Hptr_nextVer" ∷ ptr ↦[Client :: "nextVer"] #obj.(next_ver) ∗
   "Hptr_nextEpoch" ∷ ptr ↦[Client :: "nextEpoch"] #obj.(next_epoch) ∗
   "%Heq_next_ep" ∷ ⌜ length ms = uint.nat obj.(next_epoch) ⌝ ∗
+  "%Hlast_some" ∷ ⌜ ∀ m, last ms = Some m → is_Some m ⌝ ∗
   (* server info. *)
   "Hown_servCli" ∷ advrpc.Client.own ptr_serv_cli serv_cli ∗
-  "Hptr_servCli" ∷ ptr ↦[Client :: "servCli"] #ptr_serv_cli ∗
-  "Hptr_servSigPk" ∷ ptr ↦[Client :: "servSigPk"] (slice_val sl_serv_sig_pk) ∗
+  "#Hptr_servCli" ∷ ptr ↦[Client :: "servCli"]□ #ptr_serv_cli ∗
+  "#Hptr_servSigPk" ∷ ptr ↦[Client :: "servSigPk"]□ (slice_val sl_serv_sig_pk) ∗
   "#Hsl_servSigPk" ∷ own_slice_small sl_serv_sig_pk byteT DfracDiscarded obj.(serv_sig_pk) ∗
-  "Hptr_servVrfPk" ∷ ptr ↦[Client :: "servVrfPk"] #obj.(serv_vrf_pk).
+  "#Hptr_servVrfPk" ∷ ptr ↦[Client :: "servVrfPk"]□ #obj.(serv_vrf_pk).
+(*
+currently, mlist has option gname.
+change it so that it grabs the first two things.
+*)
 End defs.
 End Client.
 
+(* TODO: rm Module. *)
 Module clientErr.
 Record t :=
   mk {
@@ -80,11 +85,16 @@ Record t :=
   }.
 Section defs.
 Context `{!heapGS Σ}.
-Definition own (ptr : loc) (obj : t) : iProp Σ :=
+Definition own (ptr : loc) (obj : t) (pk : list w8) : iProp Σ :=
   ∃ (ptr_evid : loc),
   "Hptr_evid" ∷ ptr ↦[clientErr :: "evid"] #ptr_evid ∗
-  (* leftoff: if evid not nil, own and valid evid. *)
-  "Hptr_err" ∷ ptr ↦[clientErr :: "err"] #obj.(err).
+  "Hptr_err" ∷ ptr ↦[clientErr :: "err"] #obj.(err) ∗
+  match obj.(evid) with
+  | Some e =>
+    "Hown_evid" ∷ Evid.own ptr_evid e ∗
+    "#His_evid" ∷ is_Evid e pk
+  | None => True
+  end.
 End defs.
 End clientErr.
 
@@ -92,13 +102,11 @@ Section specs.
 Context `{!heapGS Σ, !pavG Σ}.
 
 Definition is_my_key cli_γ uid ver ep pk : iProp Σ :=
-  ∃ dig sm_γ comm label0 label1,
-  "#Hsubmap" ∷ mono_list_idx_own cli_γ (uint.nat ep) (Some (dig, sm_γ)) ∗
+  ∃ m_γ dig comm,
+  "#Hsubmap" ∷ mono_list_idx_own cli_γ (uint.nat ep) (Some (m_γ, dig)) ∗
   "#Hcomm" ∷ is_comm pk comm ∗
-  "#Hin_map_lat" ∷ (uid, ver) ↪[sm_γ]□ (Some (ep, comm)) ∗
-  "#His_label0" ∷ is_vrf uid ver label0 ∗
-  "#Hnin_map_next" ∷ (uid, word.add (W64 1) ver) ↪[sm_γ]□ None ∗
-  "#His_label1" ∷ is_vrf uid (word.add (W64 1) ver) label1.
+  "#Hin_map_lat" ∷ (uid, ver) ↪[m_γ]□ (Some (ep, comm)) ∗
+  "#Hnin_map_next" ∷ (uid, word.add (W64 1) ver) ↪[m_γ]□ None.
 
 Lemma wp_Client__Put ptr_c c sl_pk d0 (pk : list w8) :
   {{{
@@ -109,7 +117,7 @@ Lemma wp_Client__Put ptr_c c sl_pk d0 (pk : list w8) :
   {{{
     (ep : w64) ptr_err err, RET (#ep, #ptr_err);
     "Hsl_pk" ∷ own_slice_small sl_pk byteT d0 pk ∗
-    "Herr" ∷ clientErr.own ptr_err err ∗
+    "Herr" ∷ clientErr.own ptr_err err c.(Client.serv_sig_pk) ∗
     if negb err.(clientErr.err) then
       let new_c := set Client.next_ver (word.add (W64 1))
         (set Client.next_epoch (λ _, (word.add ep (W64 1))) c) in
@@ -124,10 +132,9 @@ Lemma wp_Client__Put ptr_c c sl_pk d0 (pk : list w8) :
 Proof. Admitted.
 
 Definition is_my_bound cli_γ uid ver (ep : w64) : iProp Σ :=
-  ∃ dig sm_γ label,
-  "#Hsubmap" ∷ mono_list_idx_own cli_γ (uint.nat ep) (Some (dig, sm_γ)) ∗
-  "#Hnin_map_next" ∷ (uid, ver) ↪[sm_γ]□ None ∗
-  "#His_label" ∷ is_vrf uid ver label.
+  ∃ m_γ dig,
+  "#Hsubmap" ∷ mono_list_idx_own cli_γ (uint.nat ep) (Some (m_γ, dig)) ∗
+  "#Hnin_map_next" ∷ (uid, ver) ↪[m_γ]□ None.
 
 Lemma wp_Client__SelfMon ptr_c c :
   {{{
@@ -136,7 +143,7 @@ Lemma wp_Client__SelfMon ptr_c c :
   Client__SelfMon #ptr_c
   {{{
     (ep : w64) ptr_err err, RET (#ep, #ptr_err);
-    "Herr" ∷ clientErr.own ptr_err err ∗
+    "Herr" ∷ clientErr.own ptr_err err c.(Client.serv_sig_pk) ∗
     if negb err.(clientErr.err) then
       let new_c := (set Client.next_epoch (λ _, (word.add ep (W64 1))) c) in
       "Hown_cli" ∷ Client.own ptr_c new_c ∗
@@ -149,18 +156,11 @@ Lemma wp_Client__SelfMon ptr_c c :
 Proof. Admitted.
 
 Definition is_other_key cli_γ uid (ep : w64) (lat : lat_val_ty) : iProp Σ :=
-  ∃ (vals : list opaque_map_val_ty) dig m_γ,
+  ∃ (vals : list opaque_map_val_ty) m_γ dig,
   "#Hpk_comm_reln" ∷ pk_comm_reln lat (last vals) ∗
-  "#Hsubmap" ∷ mono_list_idx_own cli_γ (uint.nat ep) (Some (dig, m_γ)) ∗
-  "#Hhist" ∷
-    ([∗ list] ver ↦ val ∈ vals,
-    ∃ label,
-    "#Hin_map" ∷ (uid, W64 ver) ↪[m_γ]□ Some val ∗
-    "#His_label" ∷ is_vrf uid (W64 ver) label) ∗
-  "#Hbound" ∷
-    (∃ label,
-    "#Hin_map" ∷ (uid, W64 $ length vals) ↪[m_γ]□ None ∗
-    "#His_label" ∷ is_vrf uid (W64 $ length vals) label).
+  "#Hsubmap" ∷ mono_list_idx_own cli_γ (uint.nat ep) (Some (m_γ, dig)) ∗
+  "#Hhist" ∷ ([∗ list] ver ↦ val ∈ vals, (uid, W64 ver) ↪[m_γ]□ Some val) ∗
+  "#Hbound" ∷ (uid, W64 $ length vals) ↪[m_γ]□ None.
 
 Lemma wp_Client__Get ptr_c c uid :
   {{{
@@ -170,7 +170,7 @@ Lemma wp_Client__Get ptr_c c uid :
   {{{
     (is_reg : bool) sl_pk pk (ep : w64) ep' ptr_err err,
     RET (#is_reg, slice_val sl_pk, #ep, #ptr_err);
-    "Herr" ∷ clientErr.own ptr_err err ∗
+    "Herr" ∷ clientErr.own ptr_err err c.(Client.serv_sig_pk) ∗
     if negb err.(clientErr.err) then
       let new_c := (set Client.next_epoch (λ _, word.add ep (W64 1)) c) in
       "Hown_cli" ∷ Client.own ptr_c new_c ∗
@@ -190,100 +190,202 @@ Definition is_audit (cli_γ adtr_γ : gname) (bound : w64) : iProp Σ :=
   "#Hadtr_maps" ∷ mono_list_lb_own adtr_γ ms ∗
   "%Hlen_maps" ∷ ⌜ length ms = uint.nat bound ⌝ ∗
   "%Hinv_adtr" ∷ ⌜ adtr_inv ms ⌝ ∗
-  "#Hmap_transf" ∷ (□ ∀ (ep : w64) m uid ver val dig sm_γ label,
+  "#Hmap_transf" ∷ (□ ∀ (ep : w64) m uid ver val m_γ dig,
     ("%Hlook_map" ∷ ⌜ ms !! uint.nat ep = Some m ⌝ ∗
-    "#Hsubmap" ∷ mono_list_idx_own cli_γ (uint.nat ep) (Some (dig, sm_γ)) ∗
-    "#Hin_cli" ∷ (uid, ver) ↪[sm_γ]□ val ∗
-    "#His_label" ∷ is_vrf uid ver label)
+    "#Hsubmap" ∷ mono_list_idx_own cli_γ (uint.nat ep) (Some (m_γ, dig)) ∗
+    "#Hin_cli" ∷ (uid, ver) ↪[m_γ]□ val)
     -∗
-    "%Hin_adtr" ∷ ⌜ m !! label = val ⌝).
+    (∃ label,
+    "#His_label" ∷ is_vrf uid ver label ∗
+    "%Hin_adtr" ∷ ⌜ m !! label = val ⌝)).
 
-Lemma wp_Client__auditEpoch (ep : w64) ptr_c ptr_sd sd_ptrs sd sl_serv_sig_pk (serv_sig_pk : list w8) ptr_adtr_cli adtr_cli sl_adtr_pk adtr_pk cli_dig :
+Definition auditEpoch_post adtr_pk seen_dig : iProp Σ :=
+  □ ∀ adtr_γ,
+  ("#His_pk" ∷ is_pk adtr_pk (adtr_sigpred adtr_γ))
+  -∗
+  (∃ adtr_st adtr_dig,
+  "#Hcomm_st" ∷ comm_st.valid adtr_γ adtr_st ∗
+  "%Hlook_adtr_dig" ∷ ⌜ adtr_st.(comm_st.digs) !!
+    (uint.nat seen_dig.(SigDig.Epoch)) = Some adtr_dig ⌝ ∗
+  "%Heq_dig" ∷ ⌜ seen_dig.(SigDig.Dig) = adtr_dig ⌝ ∗
+  "%Hinv" ∷ ⌜ adtr_inv adtr_st.(comm_st.key_maps) ⌝).
+
+Lemma wp_auditEpoch ptr_seen_dig seen_dig sl_serv_sig_pk (serv_sig_pk : list w8) ptr_adtr_cli adtr_cli sl_adtr_pk adtr_pk :
   {{{
-    (* cli.own sub-parts. *)
-    "Hown_sd" ∷ own_map ptr_sd (DfracOwn 1) sd_ptrs ∗
-    "Hptr_sd" ∷ ptr_c ↦[Client :: "seenDigs"] #ptr_sd ∗
-    "Hown_sd_ptrs" ∷ ([∗ map] l;v ∈ sd_ptrs;sd, SigDig.own l v) ∗
-    "Hptr_servSigPk" ∷ ptr_c ↦[Client :: "servSigPk"] (slice_val sl_serv_sig_pk) ∗
+    "#Hown_seen_dig" ∷ SigDig.own ptr_seen_dig seen_dig ∗
+    "#His_seen_dig" ∷ is_SigDig seen_dig serv_sig_pk ∗
     "#Hsl_servSigPk" ∷ own_slice_small sl_serv_sig_pk byteT DfracDiscarded serv_sig_pk ∗
-    (* the rest. *)
     "Hown_adtr_cli" ∷ advrpc.Client.own ptr_adtr_cli adtr_cli ∗
-    "#Hsl_adtrPk" ∷ own_slice_small sl_adtr_pk byteT DfracDiscarded adtr_pk ∗
-    "%His_ep" ∷ ⌜ sd !! ep = Some cli_dig ⌝
+    "#Hsl_adtrPk" ∷ own_slice_small sl_adtr_pk byteT DfracDiscarded adtr_pk
   }}}
-  Client__auditEpoch #ptr_c #ep #ptr_adtr_cli (slice_val sl_adtr_pk)
+  auditEpoch #ptr_seen_dig (slice_val sl_serv_sig_pk) #ptr_adtr_cli (slice_val sl_adtr_pk)
   {{{
     ptr_err err, RET #ptr_err;
-    "Hown_sd" ∷ own_map ptr_sd (DfracOwn 1) sd_ptrs ∗
-    "Hptr_sd" ∷ ptr_c ↦[Client :: "seenDigs"] #ptr_sd ∗
-    "Hown_sd_ptrs" ∷ ([∗ map] l;v ∈ sd_ptrs;sd, SigDig.own l v) ∗
-    "Hptr_servSigPk" ∷ ptr_c ↦[Client :: "servSigPk"] (slice_val sl_serv_sig_pk) ∗
     "Hown_adtr_cli" ∷ advrpc.Client.own ptr_adtr_cli adtr_cli ∗
-    "Herr" ∷ clientErr.own ptr_err err ∗
-    if negb err.(clientErr.err) then
-      ∀ adtr_γ,
-      ("#His_pk_adtr" ∷ is_pk adtr_pk (adtr_sigpred adtr_γ))
-      -∗
-      (∃ adtr_st adtr_dig, "#Hcomm_st" ∷ comm_st.valid adtr_γ adtr_st ∗
-      "%Hlook_adtr_dig" ∷ ⌜ adtr_st.(comm_st.digs) !! uint.nat ep = Some adtr_dig ⌝ ∗
-      "%Heq_dig" ∷ ⌜ cli_dig.(SigDig.Dig) = adtr_dig ⌝)
-    else True
+    "Herr" ∷ clientErr.own ptr_err err serv_sig_pk ∗
+    if negb err.(clientErr.err) then auditEpoch_post adtr_pk seen_dig else True
   }}}.
 Proof.
-  iIntros (Φ) "H HΦ". iNamed "H". rewrite /Client__auditEpoch.
-  wp_pures.
+  iIntros (Φ) "H HΦ". iNamed "H". iNamedSuffix "Hown_seen_dig" "_seen".
+  rewrite /auditEpoch. wp_pures.
   wp_apply wp_allocStruct; [val_ty|]. iIntros (?) "H".
   iDestruct (struct_fields_split with "H") as "H". iNamedSuffix "H" "_stdErr".
+  wp_loadField.
   wp_apply (wp_callAdtrGet with "Hown_adtr_cli"). iIntros "* H". iNamed "H".
   wp_if_destruct.
-  { iApply ("HΦ" $! _ (clientErr.mk _ _)). by iFrame "∗#". }
-  simpl. iNamed "H". iNamed "Hown_info".
+  { iApply ("HΦ" $! _ (clientErr.mk None _)). by iFrame "∗#". }
+  simpl. iNamed "H". iNamed "Hown_info". do 3 wp_loadField.
+  wp_apply wp_allocStruct; [val_ty|]. iIntros (?) "H0".
+  iMod (struct_pointsto_persist with "H0") as "#H0".
+  iDestruct (struct_fields_split with "H0") as "H1". iNamedSuffix "H1" "_serv".
+  iClear "H0". do 3 wp_loadField.
+  wp_apply wp_allocStruct; [val_ty|]. iIntros (?) "H0".
+  iMod (struct_pointsto_persist with "H0") as "#H0".
+  iDestruct (struct_fields_split with "H0") as "H1". iNamedSuffix "H1" "_adtr".
+  iClear "H0".
+  wp_apply (wp_CheckSigDig _ (SigDig.mk _ _ _) with "[]"); [iFrame "#"|].
+  iIntros (err0). iNamedSuffix 1 "_servSig". wp_if_destruct.
+  { iApply ("HΦ" $! _ (clientErr.mk None _)). by iFrame "∗#". }
+  wp_apply (wp_CheckSigDig _ (SigDig.mk _ _ _) with "[#]"); [iFrame "#"|].
+  iIntros (err1). iNamedSuffix 1 "_adtrSig". wp_if_destruct.
+  { iApply ("HΦ" $! _ (clientErr.mk None _)). by iFrame "∗#". }
+  iDestruct ("Hgenie_servSig") as "[_ H]".
+  iDestruct ("H" with "[//]") as "#His_servSig".
+  iDestruct ("Hgenie_adtrSig") as "[_ H]".
+  iDestruct ("H" with "[//]") as "#His_adtrSig".
   do 2 wp_loadField.
-  wp_apply wp_allocStruct; [val_ty|]. iIntros (?) "HservDig".
-  do 2 wp_loadField.
-  wp_apply wp_allocStruct; [val_ty|]. iIntros (?) "HadtrDig".
-  wp_loadField.
-  wp_apply (wp_CheckSigDig _ (SigDig.mk _ _ _) with "[HservDig]").
-  { iDestruct (struct_fields_split with "HservDig") as "H". iNamed "H". iFrame "∗#". }
-  iIntros (err0). iNamedSuffix 1 "_servSig".
-  wp_if_destruct.
-  { iApply ("HΦ" $! _ (clientErr.mk _ _)). by iFrame "∗#". }
-  wp_apply (wp_CheckSigDig _ (SigDig.mk _ _ _) with "[HadtrDig]").
-  { iDestruct (struct_fields_split with "HadtrDig") as "H". iNamed "H". iFrame "∗#". }
-  iIntros (err1). iNamedSuffix 1 "_adtrSig".
-  wp_if_destruct.
-  { iApply ("HΦ" $! _ (clientErr.mk _ _)). by iFrame "∗#". }
-  wp_loadField.
-  wp_apply (wp_MapGet with "Hown_sd"). iIntros (??) "[%Hlook_map Hown_sd]".
-  iDestruct (big_sepM2_lookup_r with "Hown_sd_ptrs") as (?) "[%Hlook_ptrs H]"; [exact His_ep|].
-  iNamedSuffix "H" "_cli".
-  destruct ok. 2: { exfalso. apply map_get_false in Hlook_map. set_solver. }
-  apply map_get_true in Hlook_map. simplify_eq/=.
-  wp_apply wp_Assert_true.
-  do 2 wp_loadField.
-  wp_apply (wp_BytesEqual sl_Dig sl_Dig0 with "[$Hsl_Dig $Hsl_Dig_cli]").
-  iIntros "_".
-  wp_if_destruct.
+  wp_apply (wp_BytesEqual sl_Dig0 sl_Dig with "[$Hsl_Dig $Hsl_Dig_seen]").
+  iIntros "_". wp_if_destruct.
   { wp_apply wp_allocStruct; [val_ty|]. iIntros (?) "H".
     iDestruct (struct_fields_split with "H") as "H". iNamedSuffix "H" "_evid".
-Admitted.
+    wp_apply wp_allocStruct; [val_ty|]. iIntros (?) "H".
+    iDestruct (struct_fields_split with "H") as "H". iNamedSuffix "H" "_err".
+    iApply ("HΦ" $! _ (clientErr.mk (Some
+      (Evid.mk (SigDig.mk seen_dig.(SigDig.Epoch)
+        adtrInfo.(AdtrEpochInfo.Dig) adtrInfo.(AdtrEpochInfo.ServSig))
+      seen_dig)) _)).
+    by iFrame "∗#". }
+  wp_apply wp_allocStruct; [val_ty|]. iIntros (?) "H".
+  iDestruct (struct_fields_split with "H") as "H". iNamedSuffix "H" "_err".
+  iApply ("HΦ" $! _ (clientErr.mk None _)).
+  iFrame "∗#". iIntros (?) "!>". iNamed 1.
+  iDestruct (is_sig_to_pred with "His_pk His_adtrSig") as "H".
+  iNamed "H". apply PreSigDig.inj in Henc as <-. by iFrame "#%".
+Qed.
 
-Lemma wp_Client__Audit ptr_c c (adtrAddr : w64) sl_adtrPk adtrPk :
+Lemma mono_list_lb_idx_lookup γ l i a :
+  (i < length l)%nat →
+  mono_list_lb_own γ l -∗ mono_list_idx_own γ i a -∗ ⌜ l !! i = Some a ⌝.
+Proof.
+  iIntros (?) "Hlb0". iDestruct 1 as (??) "Hlb1".
+  iDestruct (mono_list_lb_valid with "Hlb0 Hlb1") as %[Hpre|Hpre].
+  - by rewrite (prefix_lookup_lt _ _ _ _ Hpre).
+  - iPureIntro. by eapply prefix_lookup_Some.
+Qed.
+
+Lemma adtr_inv_prefix {l} l' :
+  l' `prefix_of` l →
+  adtr_inv l →
+  adtr_inv l'.
+Proof. Admitted.
+
+Lemma wp_Client__Audit ptr_c c (adtrAddr : w64) sl_adtrPk adtr_pk :
+  uint.Z c.(Client.next_epoch) > 0 →
   {{{
     "Hown_cli" ∷ Client.own ptr_c c ∗
-    "#Hsl_adtrPk" ∷ own_slice_small sl_adtrPk byteT DfracDiscarded adtrPk
+    "#Hsl_adtrPk" ∷ own_slice_small sl_adtrPk byteT DfracDiscarded adtr_pk
   }}}
   Client__Audit #ptr_c #adtrAddr (slice_val sl_adtrPk)
   {{{
     ptr_err err, RET #ptr_err;
     "Hown_cli" ∷ Client.own ptr_c c ∗
-    "Herr" ∷ clientErr.own ptr_err err ∗
+    "Herr" ∷ clientErr.own ptr_err err c.(Client.serv_sig_pk) ∗
     if negb err.(clientErr.err) then
-      "Hcan_audit" ∷ (∀ adtr_γ, is_pk adtrPk (adtr_sigpred adtr_γ) -∗
-        ("#His_audit" ∷ is_audit c.(Client.γ) adtr_γ c.(Client.next_epoch)))
+      ∀ adtr_γ,
+      ("#His_pk" ∷ is_pk adtr_pk (adtr_sigpred adtr_γ))
+      -∗
+      ("#His_audit" ∷ is_audit c.(Client.γ) adtr_γ c.(Client.next_epoch))
     else True
   }}}.
-Proof. Admitted.
+Proof.
+  iIntros (? Φ) "H HΦ". iNamed "H". rewrite /Client__Audit.
+  wp_apply wp_Dial. iIntros (??). iNamedSuffix 1 "_adtr".
+  wp_apply wp_allocStruct; [val_ty|]. iIntros (?) "Herr0".
+  wp_apply wp_ref_to; [val_ty|]. iIntros (ptr2_err0) "Hptr_err0".
+  iNamed "Hown_cli". wp_loadField.
+  wp_apply (wp_MapIter_fold _ _ _
+    (λ sd_ptrs',
+    ∃ ptr_err0 err0,
+    "Hown_cli_adtr" ∷ advrpc.Client.own ptr_cli cli ∗
+    "Herr" ∷ clientErr.own ptr_err0 err0 c.(Client.serv_sig_pk) ∗
+    "Hptr_err0" ∷ ptr2_err0 ↦[ptrT] #ptr_err0 ∗
+    if negb err0.(clientErr.err) then
+      ∃ sd',
+      "%Hdom" ∷ ⌜ dom sd_ptrs' = dom sd' ⌝ ∗
+      "%Hsub" ∷ ⌜ sd' ⊆ sd ⌝ ∗
+      "#Hpost" ∷ ([∗ map] x ∈ sd', auditEpoch_post adtr_pk x)
+    else True)%I with "Hown_sd_map [$Hown_cli_adtr $Hptr_err0 Herr0]").
+  { iDestruct (struct_fields_split with "Herr0") as "H". iNamed "H".
+    iExists (clientErr.mk None false). iFrame. iExists ∅.
+    iSplit; [done|]. iSplit. { iPureIntro. by eapply empty_subseteq. }
+    naive_solver. }
+  { clear. iIntros (??? Φ) "!> (Hpre&_&%Hlook_ptr) HΦ". iNamed "Hpre".
+    wp_loadField.
+    iDestruct (big_sepM2_lookup_l with "Hown_sd") as (?) "[%Hlook_dig Hown_dig]"; [exact Hlook_ptr|].
+    iDestruct (big_sepM_lookup with "His_sd") as "H"; [exact Hlook_dig|].
+    iNamed "H". wp_apply (wp_auditEpoch with "[$Hown_cli_adtr]"); [iFrame "#"|].
+    iIntros (??) "Haudit". iNamedSuffix "Haudit" "1".
+    iDestruct "Haudit" as "#Haudit".
+    iNamedSuffix "Herr1" "1". wp_loadField. wp_if_destruct.
+    - wp_store. iApply "HΦ". iExists ptr_err, err.
+      rewrite /clientErr.own Heqb. by iFrame "∗#".
+    - iApply "HΦ". iExists ptr_err0, err0.
+      destruct err0.(clientErr.err) eqn:Heq_err0.
+      + rewrite /clientErr.own Heq_err0. by iFrame "∗#".
+      + rewrite /clientErr.own Heq_err0. iFrame.
+        iNamedSuffix "Hpre" "_pre". iExists (<[k:=x2]>sd').
+        iIntros "!>". iSplit. { iPureIntro. set_solver. }
+        iSplit. { iPureIntro. by apply insert_subseteq_l. }
+        iApply big_sepM_insert_2; iFrame "#". }
+  iIntros "[Hown_sd_maps Hpost]". iNamed "Hpost". iClear "Hown_cli_adtr".
+  iDestruct (mono_list_lb_own_get with "Hown_epochs") as "#His_epochs".
+  wp_load. iApply "HΦ". iFrame "∗#%".
+  destruct err0.(clientErr.err); [done|].
+  iIntros "!>". iIntros (?). iNamed 1. iNamed "Hpost".
+  iDestruct (big_sepM2_dom with "Hown_sd") as %Hdom1.
+  opose proof (map_subset_dom_eq _ _ _ _ _ Hsub) as ->.
+  { by rewrite -Hdom -Hdom1. }
+
+  (* process last ep to fill is_audit adtr maps. *)
+  destruct (last ms) eqn:Hlast; rewrite last_lookup in Hlast.
+  2: { exfalso. rewrite lookup_ge_None in Hlast. word. }
+  opose proof (Hlast_some _ _) as [[[??]?]?]; [done|]. simplify_eq/=.
+  rewrite Heq_next_ep in Hlast.
+  replace (pred (uint.nat c.(Client.next_epoch))) with
+    (Z.to_nat (uint.Z c.(Client.next_epoch) - 1%Z)) in Hlast; [|word].
+  iDestruct (big_sepL_lookup with "His_maps") as "H"; [exact Hlast|]. iNamed "H".
+  iDestruct (big_sepM_lookup with "Hpost") as "H"; [exact Hlook_sd|].
+  iSpecialize ("H" with "His_pk"). iNamed "H". iNamed "Hcomm_st".
+  iDestruct (big_sepM_lookup with "His_sd") as "H"; [exact Hlook_sd|].
+  iNamed "H".
+
+  iExists (take (uint.nat c.(Client.next_epoch)) adtr_st.(comm_st.key_maps)).
+  iSplit. { iApply (mono_list_lb_own_le with "Hmaps"). apply prefix_take. }
+  iDestruct (big_sepL2_length with "Hdigs") as %?.
+  iSplit.
+  { iPureIntro. apply lookup_lt_Some in Hlook_adtr_dig.
+    rewrite Heq_ep in Hlook_adtr_dig. rewrite length_take_le; [done|word]. }
+  iSplit. { iPureIntro. refine (adtr_inv_prefix _ _ Hinv). apply prefix_take. }
+  iIntros "!> *". iNamed 1.
+
+  (* process the ep in the wand precond. *)
+  (*
+  iDestruct (mono_list_lb_idx_lookup with "His_epochs Hsubmap") as "H".
+  { apply lookup_lt_Some in Hlook_map. rewrite length_take in Hlook_map.
+    rewrite length_fmap. word. }
+    *)
+  iClear (Hlook_sd Heq_sd_dig Hlook_adtr_dig Heq_dig Hinv Heq_ep) "His_dig".
+Admitted.
 
 Lemma wp_newClient (uid servAddr : w64) sl_servSigPk servSigPk (servVrfPk : loc) :
   {{{
@@ -294,7 +396,10 @@ Lemma wp_newClient (uid servAddr : w64) sl_servSigPk servSigPk (servVrfPk : loc)
     ptr_cli cli_γ r1 r2, RET #ptr_cli;
     "Hown_cli" ∷ Client.own ptr_cli (Client.mk cli_γ uid (W64 0) (W64 0) r1 servSigPk r2)
   }}}.
-Proof. Admitted.
+Proof.
+
+(* TODO: wanna know how hard it is to prove wand.
+there might be gotchas. *)
 
 End specs.
 
