src/program_proof/pav/evidence.v
@@ -13,9 +13,9 @@ Section defs.
 Context `{!heapGS Σ, !pavG Σ}.
 Definition own ptr obj : iProp Σ :=
   ∃ ptr_sigDig0 ptr_sigDig1,
-  "Hown_sigDig0" ∷ SigDig.own ptr_sigDig0 obj.(sigDig0) ∗
+  "#Hown_sigDig0" ∷ SigDig.own ptr_sigDig0 obj.(sigDig0) ∗
   "Hptr_sigDig0" ∷ ptr ↦[Evid :: "sigDig0"] #ptr_sigDig0 ∗
-  "Hown_sigDig1" ∷ SigDig.own ptr_sigDig1 obj.(sigDig1) ∗
+  "#Hown_sigDig1" ∷ SigDig.own ptr_sigDig1 obj.(sigDig1) ∗
   "Hptr_sigDig1" ∷ ptr ↦[Evid :: "sigDig1"] #ptr_sigDig1.
 End defs.
 End Evid.
@@ -27,8 +27,12 @@ Definition is_SigDig obj pk : iProp Σ :=
   is_sig pk (PreSigDig.encodesF (PreSigDig.mk obj.(SigDig.Epoch) obj.(SigDig.Dig))) obj.(SigDig.Sig).
 
 Definition is_Evid obj pk : iProp Σ :=
-  "His_sigDig0" ∷ is_SigDig obj.(Evid.sigDig0) pk ∗
-  "His_sigDig1" ∷ is_SigDig obj.(Evid.sigDig1) pk.
+  "#His_sigDig0" ∷ is_SigDig obj.(Evid.sigDig0) pk ∗
+  "#His_sigDig1" ∷ is_SigDig obj.(Evid.sigDig1) pk ∗
+  "%Heq_ep" ∷ ⌜ obj.(Evid.sigDig0).(SigDig.Epoch) =
+                obj.(Evid.sigDig1).(SigDig.Epoch) ⌝ ∗
+  "%Hneq_dig" ∷ ⌜ obj.(Evid.sigDig0).(SigDig.Dig) ≠
+                  obj.(Evid.sigDig1).(SigDig.Dig) ⌝.
 End defs.
 
 Section wps.
@@ -36,13 +40,12 @@ Context `{!heapGS Σ, !pavG Σ}.
 
 Lemma wp_CheckSigDig ptr obj sl_pk pk :
   {{{
-    "Hown_SigDig" ∷ SigDig.own ptr obj ∗
+    "#Hown_SigDig" ∷ SigDig.own ptr obj ∗
     "#Hsl_pk" ∷ own_slice_small sl_pk byteT DfracDiscarded pk
   }}}
   CheckSigDig #ptr (slice_val sl_pk)
   {{{
     (err : bool), RET #err;
-    "Hown_SigDig" ∷ SigDig.own ptr obj ∗
     "Hgenie" ∷ (is_SigDig obj pk ∗-∗ ⌜ err = false ⌝)
   }}}.
 Proof. Admitted.
