src/program_proof/pav/auditor.v
@@ -1,7 +1,7 @@
 From Perennial.program_proof Require Import grove_prelude.
 From Goose.github_com.mit_pdos.pav Require Import kt.
 
-From Perennial.program_proof.pav Require Import core cryptoffi merkle serde server.
+From Perennial.program_proof.pav Require Import core cryptoffi merkle serde.
 
 Definition lower_adtr (m : adtr_map_ty) : merkle_map_ty :=
   (λ v, MapValPre.encodesF (MapValPre.mk v.1 v.2)) <$> m.
